# 算法导论30.2

30.2-1 Based on equation 30.6, $\omega^{n/2}_n=\omega_2$，$\omega_2=e^{\pi i}=-1$.
30.2-2 $(6, -2-2i, -2, -2+2i)$
30.2-3

```kotlin
    fun recursiveFft(): ValuePolynomial {
        val s = extendToRegular()
        val o = s.order
        if (o == 1)
            return ValuePolynomial(1) { s[0] }
        val delta = pow(E, 2.toDouble()*PI*I/o)
        var omega = complex(1.0, 0.0)
        val a0 = CoefficientPolynomial(o/2) { s[it*2] }
        val a1 = CoefficientPolynomial(o/2) { s[it*2+1] }
        val y0 = a0.recursiveFft()
        val y1 = a1.recursiveFft()
        val y = ValuePolynomial(o)
        for (k in 0 until o/2) {
            val yk = y1[k] * omega
            y[k] = y0[k] + yk
            y[k+o/2] = y0[k] - yk
            omega *= delta
        }
        return y
    }

    private fun innerReverseRecursiveFft(divideByCount: Boolean = false) : CoefficientPolynomial {
        if (count == 1)
            return CoefficientPolynomial(1) { this[0] }
        val delta = pow(E, -(2.toDouble()*PI*I/count))
        var omega = complex(1.0, 0.0)
        val a0 = ValuePolynomial(count/2) { this[it*2] }
        val a1 = ValuePolynomial(count/2) { this[it*2+1] }
        val y0 = a0.innerReverseRecursiveFft()
        val y1 = a1.innerReverseRecursiveFft()
        val y = CoefficientPolynomial(count)
        for (k in 0 until count/2) {
            val yk = y1[k] * omega
            if (divideByCount) {
                y[k] = (y0[k] + yk) / count
                y[k+count/2] = (y0[k] - yk) / count
            }
            else {
                y[k] = (y0[k] + yk)
                y[k + count / 2] = (y0[k] - yk)
            }
            omega *= delta
        }
        return y
    }
    fun inverseRecursiveFft(): CoefficientPolynomial {
        return (innerReverseRecursiveFft(true))
    }
```

View full source code on [Github](https://github.com/AaronSong321/kotlin-algorithms/tree/master/src/ds/ComplexMatrix.kt).

30.2-4 Contained in 30.2-3.
30.2-5 How many sub-questions you divde the primitive questions into never matters in the calculation of the time complexity.
First of all, expand the primitive coefficient polynomial into one with a degree divided by 3, then the recurrence equation should be
$$
A^{[0]}(x)=\sum_{i=0}^{n/3-1} a_{3i}x^i\\
A^{[1]}(x)=\sum_{i=0}^{n/3-1} a_{3i+1}x^i\\
A^{[2]}(x)=\sum_{i=0}^{n/3-1} a_{3i+2}x^i
$$
, then
$$
A(x)=A^{[0]}(x^3)+A^{[1]}(x^3)+A^{[2]}(x^3)
$$
. So the time complexity equation is
$$
T(n)=3T(n/3)+4(n/3-1)=3T(n/3)+\Theta(n)
$$. The solution is $$
T(n)=n\log n
$$ according to the master's maxim.
